Some WIP on Rewiter correctness

src/Experiments/NewPipeline/RewriterProofs.v
@@ -27,16 +27,112 @@ Module Compilers.
   Module Import RewriteRules.
     Import Rewriter.Compilers.RewriteRules.
 
+    (*
+    Module Compile.
+      Import Rewriter.Compilers.RewriteRules.Compile.
+
+      Section with_var0.
+        Context {base_type} {ident var : type.type base_type -> Type}.
+        Local Notation type := (type.type base_type).
+        Local Notation expr := (@expr.expr base_type ident var).
+        Local Notation UnderLets := (@UnderLets.UnderLets base_type ident var).
+        Let type_base (t : base_type) : type := type.base t.
+        Coercion type_base : base_type >-> type.
+      End with_var0.
+
+      Section full.
+        Context {var : type.type base.type -> Type}.
+        Local Notation expr := (@expr base.type ident).
+        Local Notation value := (@Compile.value base.type ident var).
+        Local Notation value_with_lets := (@Compile.value_with_lets base.type ident var).
+        Local Notation UnderLets := (UnderLets.UnderLets base.type ident var).
+        Local Notation reify_and_let_binds_cps := (@Compile.reify_and_let_binds_cps ident var (@UnderLets.reify_and_let_binds_base_cps var)).
+        Local Notation reflect := (@Compile.reflect ident var).
+        (*
+        Section with_rewrite_head.
+          Context (rewrite_head : forall t (idc : ident t), value_with_lets t).
+
+        End with_rewrite_head.
+
+        Notation nbe := (@rewrite_bottomup (fun t idc => reflect (expr.Ident idc))).
+
+        Fixpoint repeat_rewrite
+                 (rewrite_head : forall (do_again : forall t : base.type, @expr value (type.base t) -> UnderLets (@expr var (type.base t)))
+                                            t (idc : ident t), value_with_lets t)
+                 (fuel : nat) {t} e : value_with_lets t
+          := @rewrite_bottomup
+               (rewrite_head
+                  (fun t' e'
+                   => match fuel with
+                      | Datatypes.O => nbe e'
+                      | Datatypes.S fuel' => @repeat_rewrite rewrite_head fuel' (type.base t') e'
+                      end%under_lets))
+               t e.
+
+        Definition rewrite rewrite_head fuel {t} e : expr t
+          := reify (@repeat_rewrite rewrite_head fuel t e).*)
+
+      End full.
+
+
+      About Rewrite.
+
+      Section all.
+        Import defaults.
+        Local Notation UnderLets := (UnderLets.UnderLets base.type ident).
+
+        Context (rewrite_head : forall var (do_again : forall t, @expr (@value _ ident var) (type.base t) -> UnderLets var (@expr var (type.base t))) t,
+                    ident t -> @value_with_lets _ ident var t).
+
+
+        (*
+        Lemma Wf_Rewrite fuel {t} (e : Expr t) (Hwf : Wf e) : Wf (Rewrite rewrite_head fuel e).
+        Proof.
+          cbv [Rewrite]; intros ? ?.*)
+      End all.
+    End Compile.
+    *)
+
+    Lemma nbe_rewrite_head_eq : @nbe_rewrite_head = @nbe_rewrite_head0.
+    Proof. reflexivity. Qed.
+
+    Lemma fancy_rewrite_head_eq invert_low invert_high
+      : (fun var do_again => @fancy_rewrite_head invert_low invert_high var)
+        = (fun var => @fancy_rewrite_head0 var invert_low invert_high).
+    Proof. reflexivity. Qed.
+
+    Lemma arith_rewrite_head_eq max_const_val : @arith_rewrite_head max_const_val = (fun var => @arith_rewrite_head0 var max_const_val).
+    Proof. reflexivity. Qed.
+
+    Lemma nbe_all_rewrite_rules_eq : @nbe_all_rewrite_rules = @nbe_rewrite_rules.
+    Proof. reflexivity. Qed.
+
+    Lemma fancy_all_rewrite_rules_eq : @fancy_all_rewrite_rules = @fancy_rewrite_rules.
+    Proof. reflexivity. Qed.
+
+    Lemma arith_all_rewrite_rules_eq : @arith_all_rewrite_rules = @arith_rewrite_rules.
+    Proof. reflexivity. Qed.
+
     Lemma Wf_RewriteNBE {t} e (Hwf : Wf e) : Wf (@RewriteNBE t e).
+    Proof.
+      cbv [RewriteNBE]; rewrite nbe_rewrite_head_eq; cbv [nbe_rewrite_head0]; rewrite nbe_all_rewrite_rules_eq.
     Admitted.
     Lemma Wf_RewriteArith (max_const_val : Z) {t} e (Hwf : Wf e) : Wf (@RewriteArith max_const_val t e).
+    Proof.
+      cbv [RewriteArith]; rewrite arith_rewrite_head_eq; cbv [arith_rewrite_head0]; rewrite arith_all_rewrite_rules_eq.
     Admitted.
     Lemma Wf_RewriteToFancy (invert_low invert_high : Z -> Z -> option Z) {t} e (Hwf : Wf e) : Wf (@RewriteToFancy invert_low invert_high t e).
+    Proof.
+      cbv [RewriteToFancy]; rewrite fancy_rewrite_head_eq; cbv [fancy_rewrite_head0]; rewrite fancy_all_rewrite_rules_eq.
     Admitted.
 
     Lemma Interp_RewriteNBE {t} e (Hwf : Wf e) : Interp (@RewriteNBE t e) == Interp e.
+    Proof.
+      cbv [RewriteNBE]; rewrite nbe_rewrite_head_eq; cbv [nbe_rewrite_head0]; rewrite nbe_all_rewrite_rules_eq.
     Admitted.
     Lemma Interp_RewriteArith (max_const_val : Z) {t} e (Hwf : Wf e) : Interp (@RewriteArith max_const_val t e) == Interp e.
+    Proof.
+      cbv [RewriteArith]; rewrite arith_rewrite_head_eq; cbv [arith_rewrite_head0]; rewrite arith_all_rewrite_rules_eq.
     Admitted.
 
     Lemma Interp_RewriteToFancy (invert_low invert_high : Z -> Z -> option Z)
@@ -44,6 +140,8 @@ Module Compilers.
           (Hhigh : forall s v v', invert_high s v = Some v' -> v = Z.shiftr v' (s/2))
           {t} e (Hwf : Wf e)
       : Interp (@RewriteToFancy invert_low invert_high t e) == Interp e.
+    Proof.
+      cbv [RewriteToFancy]; rewrite fancy_rewrite_head_eq; cbv [fancy_rewrite_head0]; rewrite fancy_all_rewrite_rules_eq.
     Admitted.
   End RewriteRules.
 
